compiler/backend/passes/proofs/pure_inline_cexpProofScript.sml
@@ -492,6 +492,8 @@ Proof
     \\ irule_at Any memory_inv_APPEND \\ fs []
     \\ qpat_x_assum ‘no_shadowing _’ mp_tac
     \\ simp [Once no_shadowing_cases] \\ strip_tac
+    \\ ‘cheap x’ by (imp_res_tac specialise_is_Lam \\ simp [cheap_def])
+    \\ once_rewrite_tac [DISJOINT_SYM] \\ asm_rewrite_tac []
     \\ cheat
   )
   >~ [`Lam _ _`] >- (
