compiler/backend/passes/pure_inline_cexpScript.sml
@@ -266,32 +266,6 @@ Termination
   \\ qspec_then ‘bs’ assume_tac size_lemma \\ fs []
 End
 
-Definition boundvars_of_def:
-  boundvars_of (Var c x) = empty_vars ∧
-  boundvars_of (Prim c cop ces) =
-   FOLDR (λce s. var_union s $ boundvars_of ce) empty_vars ces ∧
-  boundvars_of (App c ce ces) =
-   FOLDR (λce s. var_union s $ boundvars_of ce) (boundvars_of ce) ces ∧
-  boundvars_of (Lam c xs ce) = insert_vars (boundvars_of ce) xs ∧
-  boundvars_of (Let c x ce1 ce2) =
-    insert_var (var_union (boundvars_of ce1) (boundvars_of ce2)) x ∧
-  boundvars_of (Letrec c fns ce) =
-    FOLDR (λ(f,body) s. var_union s $ insert_var (boundvars_of body) f)
-      (boundvars_of ce) fns ∧
-  boundvars_of (Case c ce x css us) =
-    var_union (insert_var (boundvars_of ce) x) $
-    var_union (case us of NONE => empty_vars | SOME (_,ce) => boundvars_of ce) $
-    FOLDR (λ(cn,vs,ce) s. var_union s $ insert_vars (boundvars_of ce) vs)
-      empty_vars css ∧
-  boundvars_of (NestedCase c ce x p pce pces) =
-    var_union (insert_var (boundvars_of ce) x) $
-    var_union (insert_vars (boundvars_of pce) (cepat_vars_l p)) $
-    FOLDR (λ(p,ce) s. var_union s $ insert_vars (boundvars_of ce) (cepat_vars_l p))
-      empty_vars pces
-Termination
-  WF_REL_TAC `measure $ cexp_size (K 0)`
-End
-
 Definition inline_all_def:
   inline_all cl h e =
     let (e1, s) = freshen_cexp e (boundvars_of e)
